porting simple.v to sep_buftxn

src/program_proof/simple/simple.v
@@ -6,7 +6,8 @@ From Perennial.Helpers Require Import Transitions.
 From Perennial.program_proof Require Import proof_prelude.
 
 From Goose.github_com.mit_pdos.goose_nfsd Require Import simple.
-From Perennial.program_proof Require Import txn.txn_proof buftxn.buftxn_proof marshal_proof addr_proof lockmap_proof addr.addr_proof buf.buf_proof.
+From Perennial.program_proof Require Import txn.txn_proof marshal_proof addr_proof lockmap_proof addr.addr_proof buf.buf_proof.
+From Perennial.program_proof Require Import buftxn.sep_buftxn_proof.
 From Perennial.program_proof Require Import proof_prelude.
 From Perennial.program_proof Require Import disk_lib.
 From Perennial.Helpers Require Import NamedProps Map List range_set.
@@ -21,7 +22,7 @@ Context `{!ghost_varG Σ (gmap u64 (async (list u8)))}.
 Implicit Types (stk:stuckness) (E: coPset).
 
 Record simple_names := {
-  simple_txn : @txn_names Σ;
+  simple_buftxn : buftxn_names Σ;
   simple_state : gname;
   simple_src : gen_heapG u64 (async (list u8)) Σ;
   simple_lockmapghs : list (gen_heapG u64 bool Σ);
@@ -51,13 +52,13 @@ Definition blk2addr blk := Build_addr blk 0.
 Definition is_inode_enc γ (inum: u64) (len: u64) (blk: u64) : iProp Σ :=
   ∃ (ibuf : defs.inode_buf),
     "%Hinode_encodes" ∷ ⌜ encodes_inode len blk (vec_to_list ibuf) ⌝ ∗
-    "Hinode_enc_mapsto" ∷ mapsto_txn γ.(simple_txn) (inum2addr inum) (existT _ (defs.bufInode ibuf)).
+    "Hinode_enc_mapsto" ∷ mapsto_txn γ.(simple_buftxn).(buftxn_txn_names) (inum2addr inum) (existT _ (defs.bufInode ibuf)).
 
 Definition is_inode_data γ (len : u64) (blk: u64) (contents: list u8) : iProp Σ :=
   ∃ (bbuf : Block),
     "%Hdiskdata" ∷ ⌜ firstn (length contents) (vec_to_list bbuf) = contents ⌝ ∗
     "%Hdisklen" ∷ ⌜ len = length contents ⌝ ∗
-    "Hdiskblk" ∷ mapsto_txn γ.(simple_txn) (blk2addr blk) (existT _ (defs.bufBlock bbuf)).
+    "Hdiskblk" ∷ mapsto_txn γ.(simple_buftxn).(buftxn_txn_names) (blk2addr blk) (existT _ (defs.bufBlock bbuf)).
 
 Definition is_inode_disk γ (inum: u64) (state: list u8) : iProp Σ :=
   ∃ (blk: u64),
@@ -107,31 +108,62 @@ Qed.
 Definition covered_inodes : gset u64 :=
   rangeSet 2 (NumInodes-2).
 
-Theorem wp_ReadInode γ (inum : u64) len blk (btxn : loc) bufm :
-  {{{ is_buftxn btxn bufm γ.(simple_txn) ∗
-      is_inode_enc γ inum len blk ∗
+Definition Nbuftxn := nroot .@ "buftxn".
+
+Theorem wp_ReadInode γ γtxn (inum : u64) len blk (btxn : loc) dinit P0 txn_start ibuf :
+  {{{ is_buftxn_at_txn Nbuftxn btxn γ.(simple_buftxn) dinit γtxn P0 txn_start ∗
+      buftxn_maps_to γtxn (inum2addr inum) (existT KindInode (bufInode ibuf)) ∗
+      ⌜encodes_inode len blk ibuf⌝ ∗
       ⌜ inum ∈ covered_inodes ⌝ }}}
     ReadInode #btxn #inum
   {{{ l, RET #l;
-      is_buftxn btxn bufm γ.(simple_txn) ∗
-      is_inode_enc γ inum len blk ∗
+      is_buftxn_at_txn Nbuftxn btxn γ.(simple_buftxn) dinit γtxn P0 txn_start ∗
+      buftxn_maps_to γtxn (inum2addr inum) (existT KindInode (bufInode ibuf)) ∗
       is_inode_mem l inum len blk }}}.
 Proof.
-  iIntros (Φ) "(Hbuftxn & Henc & %) HΦ".
+  iIntros (Φ) "(Hbuftxn & Henc & % & %) HΦ".
 
   wp_call.
   wp_apply (wp_inum2Addr); auto.
-(*
-  replace (#(LitInt (word.mul 128 8))) with (#1024%nat) by reflexivity.
-  wp_apply (wp_BufTxn__ReadBuf with "[$Hbuftxn]").
-*)
+  {
+    iPureIntro.
+    rewrite /covered_inodes in H1.
+    eapply rangeSet_lookup in H1; try lia.
+    rewrite /NumInodes /InodeSz. simpl. lia.
+  }
 
-  (* Need the [is_inode_enc] to be actually lifted into the buftxn active transaction.
-   * Need to solve two problems to get there:
-   * - Current buftxn spec just has a gmap, and
-   * - [is_inode_enc] is not parameterized by txn/buftxn.
-   *)
-Admitted.
+  replace (#(LitInt (word.mul 128 8))) with (#1024%nat) by reflexivity.
+  wp_apply (wp_BufTxn__ReadBuf with "[$Hbuftxn $Henc]"); eauto.
+  iIntros (dirty bufptr) "[Hbuf Hbufdone]".
+
+  wp_pures. wp_call.
+  Search _ struct.alloc.
+  wp_apply wp_allocStruct; eauto.
+  iIntros (iptr) "Hi".
+  iDestruct (struct_fields_split with "Hi") as "Hi". iNamed "Hi".
+  wp_apply (wp_buf_loadField_data with "Hbuf").
+  iIntros (bufslice) "[Hbufdata Hbufwithoutdata]".
+  rewrite is_buf_data_has_obj. iDestruct "Hbufdata" as (bufdata) "[Hbufslice %]".
+  wp_apply (wp_new_dec with "Hbufslice").
+  { rewrite /encodes_inode in H0.
+    rewrite /data_has_obj /= in H2. subst. eauto. }
+  iIntros (dec) "Hdec".
+  wp_storeField.
+  wp_apply (wp_Dec__GetInt with "Hdec"). iIntros "Hdec".
+  wp_storeField.
+  wp_apply (wp_Dec__GetInt with "Hdec"). iIntros "Hdec".
+  wp_storeField.
+  iDestruct (is_dec_to_is_slice_small with "Hdec") as "Hbufslice".
+  iMod ("Hbufdone" with "[Hbufslice Hbufwithoutdata] []") as "[Hbuftxn Hbuf]"; eauto.
+  {
+    iApply is_buf_return_data. iFrame.
+    iApply (data_has_obj_to_buf_data with "Hbufslice").
+    eauto.
+  }
+  wp_pures.
+  iApply "HΦ".
+  iFrame.
+Qed.
 
 Definition is_inode_stable γ (inum: u64) : iProp Σ :=
   ∃ (state: list u8),
@@ -140,28 +172,32 @@ Definition is_inode_stable γ (inum: u64) : iProp Σ :=
 
 Definition N := nroot .@ "simplenfs".
 
-Definition is_fs γ (nfs: loc) : iProp Σ :=
+Definition is_fs γ (nfs: loc) dinit : iProp Σ :=
   ∃ (txn lm : loc),
     "#Hfs_txn" ∷ readonly (nfs ↦[Nfs.S :: "t"] #txn) ∗
     "#Hfs_lm" ∷ readonly (nfs ↦[Nfs.S :: "l"] #lm) ∗
-    "#Histxn" ∷ is_txn txn γ.(simple_txn) ∗
+    "#Histxn" ∷ is_txn txn γ.(simple_buftxn).(buftxn_txn_names) dinit ∗
     "#Hislm" ∷ is_lockMap lm γ.(simple_lockmapghs) covered_inodes (is_inode_stable γ) ∗
     "#Hsrc" ∷ inv N (is_source γ).
 
-Theorem wp_Inode__Read γ ip inum len blk (btxn : loc) (offset : u64) (bytesToRead : u64) bufm contents :
-  {{{ is_buftxn btxn bufm γ.(simple_txn) ∗
+Theorem wp_Inode__Read γ γtxn ip inum len blk (btxn : loc) (offset : u64) (bytesToRead : u64) contents txn_start P0 dinit bbuf :
+  {{{ is_buftxn_at_txn Nbuftxn btxn γ.(simple_buftxn) dinit γtxn P0 txn_start ∗
       is_inode_mem ip inum len blk ∗
-      is_inode_data γ len blk contents }}}
+      ⌜ firstn (length contents) (vec_to_list bbuf) = contents ⌝ ∗
+      ⌜ len = length contents ⌝ ∗
+      buftxn_maps_to γtxn (blk2addr blk) (existT _ (defs.bufBlock bbuf))
+  }}}
     Inode__Read #ip #btxn #offset #bytesToRead
   {{{ resSlice (eof : bool) (vs : list u8), RET (slice_val resSlice, #eof);
       is_slice resSlice u8T 1 vs ∗
-      is_buftxn btxn bufm γ.(simple_txn) ∗
+      is_buftxn_at_txn Nbuftxn btxn γ.(simple_buftxn) dinit γtxn P0 txn_start ∗
       is_inode_mem ip inum len blk ∗
-      is_inode_data γ len blk contents ∗
+      buftxn_maps_to γtxn (blk2addr blk) (existT _ (defs.bufBlock bbuf)) ∗
       ⌜ firstn (length vs) (skipn (int.nat offset) contents) = vs ⌝ ∗
-      ⌜ eof = true <-> (int.nat offset + length vs ≥ int.nat len)%nat ⌝ }}}.
+      ⌜ eof = true <-> (int.nat offset + length vs ≥ int.nat len)%nat ⌝
+  }}}.
 Proof.
-  iIntros (Φ) "(Hbuftxn & Hmem & Hdata) HΦ".
+  iIntros (Φ) "(Hbuftxn & Hmem & % & % & Hdata) HΦ".
   wp_call.
   iNamed "Hmem".
   wp_loadField.
@@ -191,14 +227,9 @@ Proof.
     wp_pures.
     wp_loadField.
     wp_apply wp_block2addr.
-    iNamed "Hdata".
-    wp_apply (wp_BufTxn__ReadBuf _ _ _ _ _ (existT _ (bufBlock bbuf)) with "[$Hbuftxn]").
-    { iPureIntro; intuition.
-      (* XXX need to get this out of "Hdiskblk" *)
-      admit.
-    }
+    wp_apply (wp_BufTxn__ReadBuf with "[$Hbuftxn $Hdata]"); first by reflexivity.
 
-    iIntros (bufptr dirty) "[Hbuf Hbufupd]".
+    iIntros (dirty bufptr) "[Hbuf Hbufupd]".
     wp_pures.
     wp_load.
     wp_pures.
@@ -255,22 +286,15 @@ Proof.
     iIntros "(HI & Hb)".
     iNamed "HI".
 
-    iMod ("Hbufupd" with "[$Hbuf]") as "Hbuftxn".
+    iMod ("Hbufupd" with "[$Hbuf] []") as "[Hbuftxn Hbuf]".
     { intuition. }
 
-    rewrite insert_id.
-    2: { admit. }
-
-    wp_pures.
     wp_apply util_proof.wp_DPrintf.
-    wp_pures.
     wp_load.
     wp_pures.
     iApply "HΦ".
     iFrame "Hdataslice Hbuftxn".
     iFrame.
-    iSplitL "Hdiskblk".
-    { iExists _. iFrame. done. }
 
     iPureIntro. intuition.
     { admit. }
@@ -332,8 +356,8 @@ Admitted.
 
 Opaque nfstypes.READ3res.S.
 
-Theorem wp_NFSPROC3_READ γ (nfs : loc) (fh : u64) (fhslice : Slice.t) (offset : u64) (count : u32) (Q : SimpleNFS.res (bool * SimpleNFS.buf) -> iProp Σ) :
-  {{{ is_fs γ nfs ∗
+Theorem wp_NFSPROC3_READ γ (nfs : loc) (fh : u64) (fhslice : Slice.t) (offset : u64) (count : u32) (Q : SimpleNFS.res (bool * SimpleNFS.buf) -> iProp Σ) dinit :
+  {{{ is_fs γ nfs dinit ∗
       is_fh fhslice fh ∗
       ∀ σ σ' r E,
         ⌜relation.denote (SimpleNFS.wrapper fh (SimpleNFS.read fh offset count)) σ σ' r⌝ -∗
@@ -365,8 +389,9 @@ Proof.
   iIntros (reply) "Hreply".
   wp_apply util_proof.wp_DPrintf.
   wp_loadField.
-  wp_apply (wp_buftxn_Begin with "Histxn").
-  iIntros (buftx) "Hbuftxn".
+  wp_apply (wp_BufTxn__Begin with "[$Histxn]").
+  { admit. }
+  iIntros (γtxn buftx) "Hbuftxn".
   wp_apply (wp_fh2ino with "Hfh").
   wp_pures.
   wp_apply (wp_validInum).
@@ -390,12 +415,33 @@ Proof.
   iIntros "[Hstable Hlocked]".
   iNamed "Hstable".
   iNamed "Hinode_disk".
-  wp_apply (wp_ReadInode with "[$Hbuftxn $Hinode_enc]"); first by auto.
-  iIntros (ip) "(Hbuftxn & Hinode_enc & Hinode_mem)".
-  wp_apply (wp_Inode__Read with "[$Hbuftxn $Hinode_mem $Hinode_data]").
-  iIntros (resSlice eof vs) "(HresSlice & Hbuftxn & Hinode_mem & Hinode_data & %Hvs & %Heof)".
-  wp_apply (wp_BufTxn__CommitWait with "[$Hbuftxn Hfupd Hinode_state]").
-  {
+
+  (* XXX weird pattern: caller gets to lift predicates into buftxn *)
+  iNamed "Hinode_enc".
+  iSpecialize ("Hbuftxn" $! 0).
+  iMod (lift_into_txn with "Hbuftxn [$Hinode_enc_mapsto] []") as "[Hinode_enc_mapsto Hbuftxn]".
+  { solve_ndisj. }
+  { (* XXX missing from inode lock invariant? *) admit. }
+
+  wp_apply (wp_ReadInode with "[$Hbuftxn $Hinode_enc_mapsto]"); first by auto.
+  iIntros (ip) "(Hbuftxn & Hinode_enc_mapsto & Hinode_mem)".
+
+  iNamed "Hinode_data".
+  iMod (lift_into_txn with "Hbuftxn [$Hdiskblk] []") as "[Hdiskblk Hbuftxn]".
+  { solve_ndisj. }
+  { admit. }
+
+  wp_apply (wp_Inode__Read with "[$Hbuftxn $Hinode_mem $Hdiskblk]").
+  { eauto. }
+  iIntros (resSlice eof vs) "(HresSlice & Hbuftxn & Hinode_mem & Hdiskblk & %Hvs & %Heof)".
+  wp_apply (wp_BufTxn__CommitWait with "[$Hbuftxn Hinode_enc_mapsto Hdiskblk]").
+  all: try solve_ndisj.
+  2: {
+    admit.
+  }
+  { admit. }
+
+(*
     iModIntro.
     iExists _.
     iSplitR.
@@ -454,6 +500,8 @@ Proof.
   iNamed "Hreply".
   wp_storeField.
   (* XXX how to do anything with [struct.fieldRef]? *)
+  admit.
+*)
   admit.
 Admitted.
 
